AP/AP/Determinacy.lean
@@ -1,5 +1,4 @@
 import AP.AP.Basic
-import AP.Temp
 
 namespace AP
 
