AP/AP/Moves.lean
@@ -1,5 +1,4 @@
 import AP.AP.WF
-import AP.Temp
 
 namespace AP
 
